yield inv failing

Test/civl/inductive-sequentialization/Easy-PC2-new.bpl
@@ -25,114 +25,81 @@ const NumParticipants:int;
 axiom NumParticipants > 0;
 
 var {:layer 0,1} locked_requests: [Pid](Set Request);
-var {:layer 0,1} participant_votes: [Pid][Request]Vote;
+var {:layer 0,1} participant_votes: [Pid][ReqId]Vote;
 var {:layer 0,1} committed_requests: (Set Request);
 
-// function {:inline} Init(req: Request, participant_votes: [Pid][Request]Vote) : bool
-// {
-// //   participant_votes == (lambda p:Pid :: (lambda r:Request  :: NULL())) 
-//   (forall p: Pid :: participant_votes[p][req] == NULL())
-// }
+
 
 function {:inline} NoOverlap(req_set: (Set Request), d: Duration) : bool
 {
     !(exists req: Request :: Set_Contains(req_set, req) && req->duration == d)
 }
 
-// yield invariant {:layer 1} YieldInit(req: Request);
-// invariant Init(req, participant_votes); 
-
-// yield invariant {:layer 2} YieldC1();
-// invariant !(exists req1: Request, req2: Request :: req1->id != req2->id && req1->duration == req2->duration && Set_Contains(committed_requests, req1) && Set_Contains(committed_requests, req2));
-
-// yield invariant {:layer 2} YieldC2();
-// invariant (forall req: Request :: Set_Contains(committed_requests, req) ==> (forall pid: Pid :: participant_votes[pid][req] == YES() && Set_Contains(locked_requests[pid], req)));
-
-// yield invariant {:layer 1} YieldC3();
-// invariant !(exists pid: Pid, req1: Request, req2: Request :: req1->id != req2->id && req1->duration == req2->duration && participant_votes[pid][req1] == YES() && participant_votes[pid][req2] == YES());
-
-// yield invariant {:layer 1} YieldC4();
+// yield invariant {:layer 1} YieldBig();
+// invariant (forall pid: Pid, req: Request :: Set_Contains(locked_requests[pid], req) <==> participant_votes[pid][req->id] == YES());
 // invariant !(exists pid: Pid, req1: Request, req2: Request :: req1->id != req2->id && req1->duration == req2->duration && Set_Contains(locked_requests[pid], req1) && Set_Contains(locked_requests[pid], req2));
+// invariant !(exists req1: Request, req2: Request :: req1->id != req2->id && req1->duration == req2->duration && Set_Contains(committed_requests, req1) && Set_Contains(committed_requests, req2));
+// invariant !(exists req: Request, pid: Pid :: Set_Contains(committed_requests, req) && !Set_Contains(locked_requests[pid], req));
 
-// yield invariant {:layer 1} YieldC5();
-// invariant (forall pid: Pid, req: Request :: Set_Contains(locked_requests[pid], req) <==> participant_votes[pid][req] == YES());
-
-
-yield invariant {:layer 1} YieldBig();
-invariant (forall pid: Pid, req: Request :: Set_Contains(locked_requests[pid], req) <==> participant_votes[pid][req] == YES());
-invariant !(exists pid: Pid, req1: Request, req2: Request :: req1->id != req2->id && req1->duration == req2->duration && Set_Contains(locked_requests[pid], req1) && Set_Contains(locked_requests[pid], req2));
-// invariant !(exists pid: Pid, req1: Request, req2: Request :: req1->id != req2->id && req1->duration == req2->duration && participant_votes[pid][req1] == YES() && participant_votes[pid][req2] == YES());
-invariant !(exists req1: Request, req2: Request :: req1->id != req2->id && req1->duration == req2->duration && Set_Contains(committed_requests, req1) && Set_Contains(committed_requests, req2));
-invariant !(exists req: Request, pid: Pid :: Set_Contains(committed_requests, req) && !Set_Contains(locked_requests[pid], req));
-
-yield invariant {:layer 1} YieldTrue();
-invariant true;
-
-yield invariant {:layer 1} YieldVoting({:linear} pid: One ParticipantPiece, req: Request);
-invariant !(exists req0:Request :: Set_Contains(locked_requests[pid->val->id], req0) && req0->id == req->id);
-invariant participant_votes[pid->val->id][req] == NULL();
-
-// function {:inline} Init2(pids:[Pid]bool) : bool
-// {
-//   pids == MapConst(true)
-// }
-
-// yield invariant {:layer 1} YieldInit2({:linear} pids: Set Pid);
-// invariant Init2(pids->val);
-
-function {:inline} ParticipantIds(): Set Pid {
-    Set((lambda {:pool "P1"} x: int :: 1 <= x && x <= NumParticipants))
-}
+// yield invariant {:layer 1} YieldVoting({:linear} piece: One ParticipantPiece);
+// invariant !(exists req0:Request :: Set_Contains(locked_requests[piece->val->id], req0) && req0->id == piece->val->val);
+// invariant participant_votes[piece->val->id][piece->val->val] == NULL();
 
 function {:inline} JParticipantIds(j: int): Set Pid {
     Set((lambda {:pool "P1"} x: int :: j <= x && x <= NumParticipants))
-}
-
-function {:inline} AllParticipantPieces(r: ReqId): Set ParticipantPiece {
-    Set((lambda {:pool "P2"} x: ParticipantPiece :: x->val == r && x->ids == ParticipantIds() && Set_Contains(x->ids, x->id)))
 }
 
 function {:inline} JParticipantPieces(r: ReqId, j: int): Set ParticipantPiece {
     Set((lambda {:pool "P2"} x: ParticipantPiece :: x->val == r && x->ids == ParticipantIds() && Set_Contains(JParticipantIds(j), x->id)))
 }
 
-yield procedure {:layer 1} coordinator({:linear_in} reqId: One ReqId, duration: Duration)
-// refines not_skip;
-// requires call YieldInit(req);
-// requires {:layer 1} (forall p: Pid :: old(participant_votes)[p][req] == NULL());
-// requires call YieldInit2(pids);
-requires call YieldBig();
-// requires pids  == lambda .. are from 1 to n;
+function {:inline} AllParticipantPieces(r: ReqId): Set ParticipantPiece {
+    Set((lambda {:pool "P2"} x: ParticipantPiece :: x->val == r && x->ids == ParticipantIds() && Set_Contains(x->ids, x->id)))
+}
+function {:inline} ParticipantIds(): Set Pid {
+    Set((lambda {:pool "P1"} x: int :: 1 <= x && x <= NumParticipants))
+}
+
+
+yield invariant {:layer 1} YieldInit({:linear} pieces: Set ParticipantPiece, req: Request);
+invariant pieces == AllParticipantPieces(req->id);
+invariant (forall p: ParticipantPiece :: Set_Contains(pieces, p) ==> participant_votes[p->id][p->val] == NULL());
+
+yield invariant {:layer 1} YieldTrue();
+invariant true;
+
+
+yield procedure {:layer 1} coordinator({:linear_in} pieces: Set ParticipantPiece, req: Request)
+requires call YieldInit(pieces, req);
+// requires call YieldBig();
+
 {
    var i: int;
    var j: int;
    var d: Decision;
    var v: Vote;
-   var {:linear} pids: Set ParticipantPiece;
-   var {:linear} pid: One ParticipantPiece;
-   var {:linear} reqId': One ReqId;
-   
-
-   reqId' := reqId;
+   var {:linear} pieces': Set ParticipantPiece;
+   var {:linear} piece: One ParticipantPiece;
+   pieces' := pieces;
+   assume false;
    d := COMMIT();
    j := 1;
-   call pids := One_To_Fractions(reqId', ParticipantIds());
-//    assert {:layer 1} pids == AllParticipantPieces(reqId'->val);
    while (j <= NumParticipants)
    invariant {:layer 1} 1 <= j && j <= NumParticipants + 1;
-   invariant {:layer 1} pids == JParticipantPieces(reqId'->val, j);
+//    invariant {:layer 1} pieces == JParticipantPieces(reqId'->val, j);
    {
-    call pid := One_Get(pids, (Fraction(reqId'->val, j, ParticipantIds())));
-    async call voting0(Request(reqId'->val, duration), pid);
+    call piece := One_Get(pieces', (Fraction(req->id, j, ParticipantIds())));
+    async call voting0(req, piece);
     j := j + 1;
    }
 
-   call YieldBig();
+//    call YieldBig();
+   call YieldTrue();
    
    i := 1;
    while (i <= NumParticipants)
    {
-    call v := receive_vote(i, Request(reqId'->val, duration));
+    call v := receive_vote(i, req->id);
     if (v == NO())
     {
     d := ABORT();
@@ -140,75 +107,85 @@ requires call YieldBig();
     i := i + 1;
    }
 
-   call YieldBig();
+   call YieldTrue();
 
-   if (d == COMMIT()) {
-        // assert {:layer 1} false;
-        // all participants said yes
-        // locked requests of all pid have req
-        // committed => locked
-        // locked has no overlaps
-        assume false;
-        // assert {:layer 1} !(exists req1: Request :: req1->id != req->id && req1->duration == req->duration && Set_Contains(committed_requests, req1));
-        call add_to_committed_requests(Request(reqId'->val, duration));
-   }
+//    call YieldBig();
+
+//    if (d == COMMIT()) {
+//         // assert {:layer 1} false;
+//         // all participants said yes
+//         // locked requests of all pid have req
+//         // committed => locked
+//         // locked has no overlaps
+//         assume false;
+//         // assert {:layer 1} !(exists req1: Request :: req1->id != req->id && req1->duration == req->duration && Set_Contains(committed_requests, req1));
+//         call add_to_committed_requests(req);
+//    }
 }
 
-async action {:layer 1} voting(req: Request, {:linear_in} pid: One ParticipantPiece)
+async action {:layer 1} voting(req: Request, {:linear_in} piece: One ParticipantPiece) //(reqid, pid) (4, 3) (5, 3)
 modifies locked_requests, participant_votes;
+asserts piece->val->val == req->id;
 // asserts !(exists req0:Request :: Set_Contains(locked_requests[pid], req0) && req0->id == req->id);
 // asserts participant_votes[pid][req] == NULL();
 {
-    assert !(exists req0:Request :: Set_Contains(locked_requests[pid->val->id], req0) && req0->id == req->id);
-    assert participant_votes[pid->val->id][req] == NULL();
-    if (*) {
-        participant_votes[pid->val->id][req] := NO();
-        return;
-    }
-    else {
-        if (NoOverlap(locked_requests[pid->val->id], req->duration)) {
-            locked_requests[pid->val->id] := Set_Add(locked_requests[pid->val->id], req);
-            participant_votes[pid->val->id][req] := YES();
+    // assert !(exists req0:Request :: Set_Contains(locked_requests[pid->val->id], req0) && req0->id == req->id);
+    // assert participant_votes[piece->val->id][piece->val->val] == NULL();
+    // if (*) {
+    //     participant_votes[pid->val->id][req] := NO();
+    //     return;
+    // }
+    // else {
+        
+        if (NoOverlap(locked_requests[piece->val->id], req->duration)) {
+            locked_requests[piece->val->id] := Set_Add(locked_requests[piece->val->id], req);
+            participant_votes[piece->val->id][req->id] := YES();
         }
         else {
-            participant_votes[pid->val->id][req] := NO();
+            participant_votes[piece->val->id][req->id] := NO();
         }
-    }
+    // }
 }
-yield procedure {:layer 0} voting1(req: Request, {:linear_in} pid: One ParticipantPiece);
+yield procedure {:layer 0} voting1(req: Request, {:linear_in} piece: One ParticipantPiece);
 refines voting;
 
-yield procedure {:layer 1} voting0(req: Request, {:linear_in}  pid: One ParticipantPiece)
-requires call YieldBig();
-requires call YieldVoting(pid, req);
+yield procedure {:layer 1} voting0(req: Request, {:linear_in}  piece: One ParticipantPiece)
+// requires call YieldBig();
+// requires call YieldVoting(piece);
 {
     // assert {:layer 1} !(exists req0:Request :: Set_Contains((locked_requests)[pid], req0) && req0->id == req->id);
     // assert {:layer 1} (participant_votes)[pid][req] == NULL();
-    call voting1(req, pid);
+    call voting1(req, piece);
 }
 
-action {:layer 1} ADD_TO_COMMITTED_REQUESTS( req: Request)
+
+
+action {:layer 1} ADD_TO_COMMITTED_REQUESTS(req: Request)
 modifies committed_requests;
 asserts !(exists req0:Request :: Set_Contains(committed_requests, req0) && req0->id == req->id);
 asserts !(exists req1: Request :: req1->id != req->id && req1->duration == req->duration && Set_Contains(committed_requests, req1));
 {
     committed_requests := Set_Add(committed_requests, req);
 }
-yield procedure {:layer 0} add_to_committed_requests( req: Request);
+yield procedure {:layer 0} add_to_committed_requests(req: Request);
 refines ADD_TO_COMMITTED_REQUESTS;
 
-right action {:layer 1} RECEIVE_VOTE(pid: Pid, req: Request) returns (v: Vote)
+
+
+right action {:layer 1} RECEIVE_VOTE(pid: Pid, reqId: ReqId) returns (v: Vote)
 {
-   assume participant_votes[pid][req] != NULL();
-   v := participant_votes[pid][req];
+   assume participant_votes[pid][reqId] != NULL();
+   v := participant_votes[pid][reqId];
 }
-yield procedure {:layer 0} receive_vote(pid: Pid,  req: Request) returns (v: Vote);
+yield procedure {:layer 0} receive_vote(pid: Pid,  reqId: ReqId) returns (v: Vote);
 refines RECEIVE_VOTE;
 
-action {:layer 1} WAIT_FOR_PARTICIPANT_VOTE( req: Request)
+
+
+action {:layer 1} WAIT_FOR_PARTICIPANT_VOTE(reqId: ReqId)
 {
-      assume (forall pid: Pid :: (1 <= pid && pid <= NumParticipants) ==> participant_votes[pid][req] != NULL());
+      assume (forall pid: Pid :: (1 <= pid && pid <= NumParticipants) ==> participant_votes[pid][reqId] != NULL());
 }
-yield procedure {:layer 0} wait_for_participant_vote( req: Request); 
+yield procedure {:layer 0} wait_for_participant_vote(reqId: ReqId); 
 refines WAIT_FOR_PARTICIPANT_VOTE;
 
